update selfbalance link and simulate to v103. remove duplicate bytecode module

RocqOfRust/revm/revm_interpreter/instructions/simulate/host/selfbalance.v
@@ -4,12 +4,12 @@ Require Import core.links.array.
 Require Import revm.revm_context_interface.links.host.
 Require Import revm.revm_context_interface.links.journaled_state.
 Require Import revm.revm_context_interface.simulate.host.
-Require Import revm.revm_interpreter.gas.simulate.constants.
 Require Import revm.revm_interpreter.instructions.links.host.selfbalance.
 Require Import revm.revm_interpreter.instructions.simulate.macros.
+Require Import revm.revm_interpreter.links.instruction_context.
 Require Import revm.revm_interpreter.links.interpreter.
-Require Import revm.revm_interpreter.links.instruction_result.
 Require Import revm.revm_interpreter.links.interpreter_types.
+Require Import revm.revm_interpreter.simulate.interpreter.
 Require Import revm.revm_interpreter.simulate.interpreter_types.
 Require Import revm.revm_primitives.links.hardfork.
 
@@ -25,25 +25,18 @@ Definition selfbalance
   check_macro interpreter SpecId.ISTANBUL
     (fun interpreter => (interpreter, host))
     (fun interpreter =>
-  gas_macro interpreter constants.LOW
-    (fun interpreter => (interpreter, host))
-    (fun interpreter =>
   let target :=
     IInterpreterTypes.(InterpreterTypes.InputsTrait_for_Input).(InputTraits.target_address)
       interpreter.(Interpreter.input) in
   let '(balance_opt, host) := IHost.(Host.balance) host target in
   match balance_opt with
   | None =>
-    let control :=
-      IInterpreterTypes.(InterpreterTypes.LoopControl_for_Control).(LoopControl.set_instruction_result)
-        interpreter.(Interpreter.control)
-        instruction_result.InstructionResult.FatalExternalError in
-    (interpreter <| Interpreter.control := control |>, host)
+    (halt_fatal interpreter, host)
   | Some balance =>
   push_macro interpreter balance.(StateLoad.data)
     (fun interpreter => (interpreter, host))
     (fun interpreter => (interpreter, host))
-  end)).
+  end).
 
 Lemma selfbalance_eq
     {WIRE H : Set} `{Link WIRE} `{Link H}
@@ -60,10 +53,14 @@ Lemma selfbalance_eq
     (host : H) :
   let ref_interpreter := make_ref 0 in
   let ref_host := make_ref (A := H) 1 in
+  let context := {|
+    instruction_context.InstructionContext.interpreter := ref_interpreter;
+    instruction_context.InstructionContext.host := ref_host;
+  |} in
   let result := selfbalance interpreter host in
   {{
     SimulateM.eval_f
-      (run_selfbalance run_InterpreterTypes_for_WIRE run_Host_for_H ref_interpreter ref_host)
+      (run_selfbalance run_InterpreterTypes_for_WIRE run_Host_for_H context)
       [interpreter; host]%stack 🌲
     (
       Output.Success tt,
@@ -71,21 +68,25 @@ Lemma selfbalance_eq
     )
   }}.
 Proof.
+  intros.
+  subst result.
   with_strategy transparent [run_selfbalance] unfold selfbalance, run_selfbalance; cbn.
   check_macro_eq InterpreterTypesEq.
-  gas_macro_eq idtac.
   s. {
     apply InterpreterTypesEq.
   }
   s. {
     apply HostEq.
   }
-  destruct _.(Host.balance) as [[balance|] ?host]; cbn. 2: {
-    s. {
-      apply InterpreterTypesEq.
-    }
+  destruct _.(Host.balance) as [[balance|] host_after]; cbn.
+  - push_macro_eq InterpreterTypesEq.
     s.
-  }
-  push_macro_eq InterpreterTypesEq.
-  s.
+  - s.
+    + apply
+        (halt_fatal_eq
+          run_InterpreterTypes_for_WIRE
+          InterpreterTypesEq
+          interpreter
+          [host_after; tt]%stack).
+    + s.
 Qed.
