RocqOfRust/revm/revm_bytecode/links/bytecode.v
@@ -34,21 +34,6 @@ Module Impl_Bytecode.
 End Impl_Bytecode.
 Export (hints) Impl_Bytecode.
 
-Module Bytecode.
-  Parameter t : Set.
-
-  Parameter to_value : t -> Value.t.
-
-  Global Instance IsLink : Link t := {
-    Φ := Ty.path "revm_bytecode::bytecode::Bytecode";
-    φ := to_value;
-  }.
-
-  Definition of_ty : OfTy.t (Ty.path "revm_bytecode::bytecode::Bytecode").
-  Proof. eapply OfTy.Make with (A := t); reflexivity. Defined.
-  Smpl Add apply of_ty : of_ty.
-End Bytecode.
-
 (* Module Bytecode.
   Inductive t : Set :=
   | LegacyAnalyzed
